\begin{enumialphparenastyle}

\begin{ex} For each matrix $A$, find the product $(-2)A, 0A,$ and $3A$. 
\begin{enumerate}
\item
$A = \begin{mymatrix}{rr}
1 & 2 \\
2 & 1 
\end{mymatrix}$

\item
$A = \begin{mymatrix}{rr}
-2 & 3 \\
0 & 2 
\end{mymatrix}$

\item
$A = \begin{mymatrix}{rrr}
0 & 1 & 2 \\
1 & -1 & 3 \\
4 & 2 & 0 
\end{mymatrix}$
\end{enumerate}
%\begin{sol}
%\end{sol}
\end{ex}

\begin{ex} \label{addinvrstunique} Using only the properties given in Proposition \ref{prop:properties-of-addition}
 and Proposition \ref{prop:properties-scalar-mult}, 
show $-A$ is unique.
\begin{sol}
 Suppose $B$ also works. Then
\[
-A=-A+\tup{A+B} =\tup{-A+A} +B=0+B=B
\]
\end{sol}
\end{ex}

\begin{ex} Using only the properties given in Proposition \ref{prop:properties-of-addition} 
and Proposition \ref{prop:properties-scalar-mult}
show $0$ is unique. 
\begin{sol}
Suppose $0^{\prime }$ also works. Then $0^{\prime }=0^{\prime }+0=0.$
\end{sol}
\end{ex}

\begin{ex} Using only the properties given in Proposition \ref{prop:properties-of-addition}
 and Proposition \ref{prop:properties-scalar-mult} show $0A=0.$ Here
the $0$ on the left is the scalar $0$ and the $0$ on the right is the zero matrix of appropriate size.
\begin{sol}
$0A=\tup{0+0} A=0A+0A.$ Now add $-\tup{
0A} $ to both sides. Then $0=0A$.
\end{sol}
\end{ex}

\begin{ex} Using only the properties given in Proposition \ref{prop:properties-of-addition} and 
Proposition \ref{prop:properties-scalar-mult}, as well as previous
problems show $\tup{-1} A=-A.$
\begin{sol}
$A+\tup{-1} A=\tup{1+\tup{
-1} } A=0A=0.$ Therefore, from the uniqueness of the additive
inverse proved in the above Problem \ref{addinvrstunique}, it follows that $
-A=\tup{-1} A$.
\end{sol}
\end{ex}

\end{enumialphparenastyle}