\section*{Exercises}


\begin{ex}
  Find $\begin{mymatrix}{c}
    1 \\
    2 \\
    3
  \end{mymatrix} +\begin{mymatrix}{c}
    1 \\
    5 \\
    1
  \end{mymatrix} +\begin{mymatrix}{c}
    -1 \\
    2 \\
    -4
  \end{mymatrix}$.
  
  \begin{sol}
    $\begin{mymatrix}{r}
      1 \\
      9 \\
      0
    \end{mymatrix}$.
  \end{sol}
\end{ex}

\begin{ex}
  Use the properties of vector addition from
  Theorem~\ref{thm:properties-vector-addition} to show the following
  equalities. Justify every step. 
  \begin{enumerate}
  \item $(\vect{u}+\vect{v})+\vect{w} = (\vect{v}+\vect{w})+\vect{u}$.
  \item $(\vect{u}+\vect{0})+(\vect{v}+(-\vect{u})) = \vect{v}$.
  \end{enumerate}

  \begin{sol}
    \begin{enumerate}
    \item
      $(\vect{u}+\vect{v})+\vect{w} = (\vect{v}+\vect{u})+\vect{w} =
      \vect{v}+(\vect{u}+\vect{w}) = \vect{v}+(\vect{w}+\vect{u}) =
      (\vect{v}+\vect{w})+\vect{u}$. Here we have used the commutative
      law, the associative law, the commutative law, and the
      associative law, in that order.
    \item
      $(\vect{u}+\vect{0})+(\vect{v}+(-\vect{u}) =
      \vect{u}+(\vect{v}+(-\vect{u}) = \vect{u}+((-\vect{u})+\vect{v})
      = (\vect{u}+(-\vect{u}))+\vect{v} = \vect{0}+\vect{v} =
      \vect{v}+\vect{0} = \vect{v}$. Here we have used the additive
      unit, the commutative law, the associative law, the additive
      inverse, the commutative law, and the additive unit, in that
      order.
    \end{enumerate}
  \end{sol}
\end{ex}

