\begin{enumialphparenastyle}

\begin{ex} Given the points $P=(2,0,-4)$ and $Q=(5,-2,1)$, find $\longvect{PQ}$ and $\longvect{QP}$.
 
\begin{sol}

\begin{equation*}
\longvect{PQ}  = \longvect{0Q} - \longvect{0P}= \begin{mymatrix}{c}
5-2\\
 -2-0 \\
1-(-4)
\end{mymatrix} = \begin{mymatrix}{c}
3\\
 -2 \\
5
\end{mymatrix}
\end{equation*}

\begin{equation*}
\longvect{QP}  = \longvect{0P} - \longvect{0Q}= \begin{mymatrix}{c}
2-5\\
 0-(-2) \\
(-4)-1
\end{mymatrix} = \begin{mymatrix}{c}
-3\\
 2 \\
-5
\end{mymatrix}
\end{equation*}

\end{sol}
\end{ex}

\begin{ex} Find $x$ and $y$ so that $\vect{u}= \begin{mymatrix}{cc}
5x-3y & 4
\end{mymatrix}$ and $\vect{v}= \begin{mymatrix}{cc}
2x-2y & 2y
\end{mymatrix}$ are equal in $\R^2$.
 
\begin{sol}

We need $5x-3y=2x-y$ and $4=2y$ we solve for $y$ first, $y=2$ then we get 
\begin{align*}
5x-3\cdot 2&=2x-2\\
3x-6&=-2\\
3x&=4\\
x&=\frac{4}{3}
\end{align*}


\begin{equation*}
\longvect{PQ}  = \longvect{0Q} - \longvect{0P}= \begin{mymatrix}{c}
5-2\\
 -2-0 \\
1-(-4)
\end{mymatrix} = \begin{mymatrix}{c}
3\\
 -2 \\
5
\end{mymatrix}
\end{equation*}

\begin{equation*}
\longvect{QP}  = \longvect{0P} - \longvect{0Q}= \begin{mymatrix}{c}
2-5\\
 0-(-2) \\
(-4)-1
\end{mymatrix} = \begin{mymatrix}{c}
-3\\
 2 \\
-5
\end{mymatrix}
\end{equation*}

\end{sol}
\end{ex}


\end{enumialphparenastyle}