\section*{Exercises}


\begin{ex} Determine which matrices are in {\rref}. 

\begin{enumerate}
\item $\begin{mymatrix}{rrr}
1 & 2 & 0 \\
0 & 1 & 7
\end{mymatrix} $

\item $\begin{mymatrix}{rrrr}
1 & 0 & 0 & 0 \\
0 & 0 & 1 & 2 \\
0 & 0 & 0 & 0
\end{mymatrix} $

\item $\begin{mymatrix}{rrrrrr}
1 & 1 & 0 & 0 & 0 & 5 \\
0 & 0 & 1 & 2 & 0 & 4 \\
0 & 0 & 0 & 0 & 1 & 3
\end{mymatrix} $
\end{enumerate}
\begin{sol}
\begin{enumerate}
\item This one is not.
\item This one is.
\item This one is.
\end{enumerate}
\end{sol}
\end{ex}

\begin{ex}
 Reduce each of the matrices from Exercise~\ref{ex:rr-ef} to {\rref}.
\end{ex}

\begin{ex} Use Gauss-Jordan elimination to solve the system of equations
$-8x+2y+5z=18,-8x+3y+5z=13$, and $-4x+y+5z=19$.
\begin{sol}
 Solution is: $\mat{x=-1,y=-5,z=4} $
\end{sol}
\end{ex}

\begin{ex} Use Gauss-Jordan elimination to solve the system of equations $3x-y-2z=3$, 
$y-4z=0$, and $-2x+y=-2$.
\begin{sol}
Solution is: $\mat{x=2t+1,y=4t,z=t} $
\end{sol}
\end{ex}

\begin{ex} Use Gauss-Jordan elimination to solve the system of equations 
$-9x+15y=66,-11x+18y=79$, $-x+y=4$, and $z=3$.
\begin{sol}
Solution is: $\mat{x=1,y=5,z=3} $
\end{sol}
\end{ex}

\begin{ex} Use Gauss-Jordan elimination to solve the system of equations $-19x+8y=-108$,
$-71x+30y=-404$, $-2x+y=-12$, $4x+z=14$.
\begin{sol}
Solution is: $\mat{x=4,y=-4,z=-2} $
\end{sol}
\end{ex}

\begin{ex}
  Solve the following two systems of equations simultaneously, by
  using a single augmented matrix with two constant vectors.
  \begin{equation*}
    \begin{array}{r@{~}c@{~}l@{~}}
      x  + 2y -  z &=& 0 \\
      2x + 3y +  z &=& 3 \\
      x  -  y + 2z &=& 3 \\
    \end{array}
    \quad\quad
    \begin{array}{r@{~}c@{~}l@{~}}
      x  + 2y -  z &=& 1 \\
      2x + 3y +  z &=& 7 \\
      x  -  y + 2z &=& 4 \\
    \end{array}
  \end{equation*}

  \begin{sol}
    The rank of the coefficient matrix is $3$, so both systems have a
    unique solution. The solution of the first system is
    $(x,y,z)=(1,0,1)$, and the solution of the second system is
    $(x,y,z)=(1,1,2)$.
  \end{sol}
\end{ex}

